theories/ok.v
@@ -1,0 +1,251 @@
+From Stdlib Require Import
+  Arith   
+  Basics         
+  Classes.RelationClasses
+  Logic.FunctionalExtensionality
+  Morphisms
+  Nat
+  Program.Basics
+  List
+  Lia.
+
+Definition proc := True.
+Definition rvar := True.
+
+Inductive EC_term :=
+| Ebag (m n:nat) (EP : EC_proc)   (* nu. {f1...fm} {r1..rn} EP *)
+
+with EC_proc :=
+| Ehol
+| Edeflam (r : rvar) (Et : EC_term)  (* r <- lam r'. Et *)
+| Epar (EP : EC_proc) (P : proc). (* EP | P *)
+(* May need left and right Epars *)
+
+
+Scheme EC_term_ind_m := Induction for EC_term Sort Prop
+  with EC_proc_ind_m := Induction for EC_proc Sort Prop.
+Combined Scheme EC_ind from EC_term_ind_m, EC_proc_ind_m.
+
+Scheme EC_term_rect_m := Induction for EC_term Sort Type
+  with EC_proc_rect_m := Induction for EC_proc Sort Type.
+Combined Scheme EC_rect from EC_term_rect_m, EC_proc_rect_m.
+
+Scheme EC_term_rec_m := Induction for EC_term Sort Set
+  with EC_proc_rec_m := Induction for EC_proc Sort Set.
+Combined Scheme EC_rec from EC_term_rec_m, EC_proc_rec_m.
+
+
+(* Projects the EC_term components *)
+Definition get_fvars_Et Et := match Et with Ebag m _ _ => m end.
+Definition get_rvars_Et Et := match Et with Ebag _ n _ => n end.
+Definition get_proc_Et Et := match Et with Ebag _ _ EP => EP end.
+
+
+
+Inductive less_Epars : EC_term -> EC_term -> Prop :=
+| top_Epar : 
+  forall (m n : nat) (EP : EC_proc) (P : proc),
+    less_Epars (Ebag m n EP) (Ebag m n (Epar EP P))
+.
+
+Lemma less_Epars_wf_helper : 
+  (forall (Et : EC_term), Acc less_Epars Et) /\
+  (forall (EP : EC_proc) m n, Acc less_Epars (Ebag m n EP)).
+Proof. 
+  apply EC_ind; intros.
+  (* Ebag is immediate by IH *)
+  - apply H.
+  (* Ehol and Edeflam are base cases: there is no Epar to remove *)
+  - constructor; intros. inversion H.
+  - constructor; intros. inversion H0.
+  (* Epar follows from IH *)
+  - constructor; intros. inversion H0; subst. apply H.
+Qed.
+
+Lemma less_Epars_wf : well_founded less_Epars.
+Proof. unfold well_founded; apply less_Epars_wf_helper. Qed.
+
+
+(* Gives the number of lambda bindings encountered when traversing 
+      to the hole (i.e. how many scopes deep the hole is) *)
+Fixpoint hole_depth Et := hole_depth_proc (get_proc_Et Et)
+with hole_depth_proc (EP : EC_proc) : nat :=
+  match EP with
+  | Ehol => 0
+  | Edeflam _ Et => 1 + hole_depth Et
+  | Epar EP' _ => hole_depth_proc EP'
+  end.
+
+Definition is_hole_scope_at_top := compose (eqb 0) hole_depth.
+Definition is_hole_scope_at_top_proc := compose (eqb 0) hole_depth_proc.
+
+(* States the hole_depth of an EC is less than another *)
+Definition hole_depth_lt (Et1 Et2 : EC_term) := 
+  lt (hole_depth Et1) (hole_depth Et2).
+
+(* Every EC is accessible with hole_depth_lt.
+   Used to prove well-foundedness of split_hole_scope. *)
+Lemma hole_depth_lt_wf_helper : 
+  (forall (Et : EC_term), Acc hole_depth_lt Et) /\
+  (forall (EP : EC_proc) m n, Acc hole_depth_lt (Ebag m n EP)).
+Proof. 
+  apply EC_ind; intros.
+  (* Ebag is immediate by IH *)
+  - apply H.
+  (* Ehol has depth 0 and is the base case *)
+  - constructor; intros. unfold hole_depth_lt in H; simpl in H. lia.
+  (* Elam adds to depth *)
+  - constructor; intros.
+    (* Case on whether we need a new Acc layer before IH *)
+    destruct (Nat.eqb_spec (hole_depth y) (hole_depth Et)).
+    + constructor; intros. apply (Acc_inv H). 
+      unfold hole_depth_lt in *. rewrite <- e. apply H1.
+    + apply (Acc_inv H). unfold hole_depth_lt in *. simpl in H0. lia.
+  (* Epar follows from IH *)
+  - constructor; intros. specialize H with m n. apply (Acc_inv H).
+    unfold hole_depth_lt in *; auto.
+Qed.
+
+Definition hole_depth_lt_OR_less_Epars :=
+  fun Et1 Et2 => hole_depth_lt Et1 Et2 \/ less_Epars Et1 Et2.
+
+(* Every EC is accessible with hole_depth_lt.
+   Used to prove well-foundedness of split_hole_scope. *)
+Lemma hole_depth_lt_OR_less_Epars_wf_helper : 
+  (forall (Et : EC_term), Acc hole_depth_lt_OR_less_Epars Et) /\
+  (forall (EP : EC_proc) m n, Acc hole_depth_lt_OR_less_Epars (Ebag m n EP)).
+Proof. 
+  unfold hole_depth_lt_OR_less_Epars, hole_depth_lt. apply EC_ind; intros.
+  (* Ebag is immediate by IH *)
+  - apply H.
+  (* Ehol has depth 0 and has no Epars *)
+  - constructor; intros.
+    simpl in H. destruct H.
+    + lia.
+    + inversion H.
+  (* Elam adds to depth but has no Epars *)
+  - constructor; intros. destruct H0.
+
+
+    + (* Case on whether we need a new Acc layer before IH *)
+      simpl in H0.
+      destruct (Nat.eqb_spec (hole_depth y) (hole_depth Et)).
+      * constructor; intros. apply (Acc_inv H).
+        rewrite <- e; clear e. destruct H1; auto.
+         admit.
+      * apply (Acc_inv H). simpl in H0. lia.
+    + inversion H0.
+  (* Epar follows from IH *)
+  - constructor; intros. destruct H0.
+    + apply (Acc_inv (H m n)). auto.
+    + inversion H0; subst. apply H.
+Admitted.
+
+
+
+Lemma hole_depth_lt_wf : well_founded hole_depth_lt.
+Proof. unfold well_founded; apply hole_depth_lt_wf_helper. Qed.
+
+Lemma hole_depth_lt_OR_less_Epars_wf : 
+  well_founded (fun Et1 Et2 => hole_depth_lt Et1 Et2 \/ less_Epars Et1 Et2).
+Proof. unfold well_founded; intros. Search well_founded. Print Nat.lt_wf. Admitted.
+
+
+
+
+
+
+(* Given an EC, pops the top scope from the next scope containing the hole
+      (if different), returning a pair whose first element is the top scope
+      and second element is the EC process containing the next scope.
+    1) If the hole is at the top scope, returns (EC, Ehol)
+    2) If the hole is under a lambda, returns (EC_top, EC_lam) where:
+        - EC_top is the EC with the lamdef replaced with a hole
+        - EC_lam is the lamdef removed from the EC
+
+  If this function takes EC and returns (EC_top, EC_next),
+    1) Filling EC_top with EC_next will give EC.
+    2) EC_next is either Ehol or Edeflam
+    3) If EC_next is Ehol, then EC_top is EC *)
+
+Fixpoint pop_EC_scope_proc (EP : EC_proc) : EC_proc * EC_proc :=
+  match EP with
+  | Ehol => (Ehol, Ehol)    (* Hole is at the top scope *)
+  | Epar EP' P => let (EP1, EP2) := pop_EC_scope_proc EP' in   (* Recurse *)
+                      (Epar EP1 P, EP2)
+  | Edeflam _ _ => (Ehol, EP)    (* Split top and next scope *)
+  end.
+
+Definition pop_EC_scope (Et : EC_term) : EC_term * EC_proc :=
+  match Et with
+  | Ebag m n EP => let (EP1, EP2) := pop_EC_scope_proc EP in   (* Recurse *)
+                      (Ebag m n EP1, EP2)
+  end.
+
+
+  
+
+(* pop_EC_scope reduces hole_depth *)
+Lemma pop_EC_scope_reduces_hole_depth :
+  forall Et Et' Et0 r,
+    pop_EC_scope Et = (Et0, Edeflam r Et') ->
+    hole_depth_lt Et' Et.
+Proof.
+  intro Et; unfold hole_depth_lt. destruct Et.
+  induction EP; intros; simpl in *.
+  - discriminate.
+  - injection H; intros. rewrite H0. apply Nat.lt_succ_diag_r.
+  - destruct (pop_EC_scope_proc EP). eapply IHEP. 
+    injection H; intros. rewrite H0; reflexivity.
+Defined.
+
+
+(* HELPER FUNCTION! ACC is the proof of accessibility for Et_cur 
+    (i.e. that the hole_depth of Et_cur decreases at each call) *)
+Fixpoint split_hole_scope_builder (r : rvar) (Et_acc Et_cur : EC_term) 
+        (ACC : Acc hole_depth_lt Et_cur) {struct ACC} : EC_term * EC_proc :=
+  (match pop_EC_scope Et_cur as y 
+      return (pop_EC_scope Et_cur = y) -> EC_term * EC_proc with
+  | (_, Ehol) => fun _ => (Et_acc, Edeflam r Et_cur)
+  | (Et_next, Edeflam r' Et_rest) => fun HEQ =>
+          let ACC_Et_rest := Acc_inv ACC 
+              (pop_EC_scope_reduces_hole_depth Et_cur Et_rest Et_next r' HEQ) in
+          split_hole_scope_builder r'
+              Et_next Et_rest ACC_Et_rest
+  | _ => fun _ => (Ebag 0 0 Ehol, Ehol) (* Cannot reach here *)
+  end) eq_refl.
+
+
+(* Applies pop_EC_scope until the "hole scope" is reached,
+      separating the hole scope from the rest of the EC.
+   Given an EC, returns a pair whose 
+      first element is the EC with the hole scope replaced by a hole
+      and second element is the hole scope.
+   The invariants of pop_EC_scope are also held by split_hole_scope. *)
+Definition split_hole_scope (Et : EC_term) : EC_term * EC_proc :=
+  match pop_EC_scope Et with
+  | (_, Ehol) => (Et, Ehol)
+  | (Et_acc, Edeflam r Et_cur) => split_hole_scope_builder r Et_acc Et_cur (hole_depth_lt_wf Et_cur)
+  | _ => (Ebag 0 0 Ehol, Ehol) (* Cannot reach here *)
+  end.
+
+
+
+
+
+Lemma inv_split_hole_scope_builder :
+  forall Et_cur r Et_acc ACC,
+    exists Et_outer r' Et_hs,
+    split_hole_scope_builder r Et_acc Et_cur ACC = 
+    (Et_outer, Edeflam r' Et_hs).
+Proof.
+  induction Et_cur using (well_founded_induction hole_depth_lt_wf).
+  destruct Et_cur; destruct EP; intros; destruct ACC.
+  - simpl. eexists; eauto.
+  - apply (H Et). unfold hole_depth_lt; auto.
+  - 
+    unfold split_hole_scope_builder. fold split_hole_scope_builder.
+    remember (Ebag m n (Epar EP P)) as x.
+    destruct (pop_EC_scope x).
+    admit.
+Admitted.
